\documentclass[12pt]{article}
\usepackage{graphicx} % Required for inserting images
\usepackage{amsmath}
\usepackage{amssymb}
%\usepackage[italian]{babel}
\usepackage{hyperref}%
\usepackage{mathrsfs}

\begin{document}

\section*{}
Marco Reina 7066486 \newline
Samuele Serri 7069839 \newline
\section*{1}
\section*{a)}
$f_1(x) = a_1 + b_1x + c_1x^2 + d_1x^3 \  \ x\leq\xi$ \newline
if $x \leq \xi$ then $(x - \xi)_{+}^3 = 0$ by definition, so we can simply set: \newline
$a_1  = \beta_0 \\ b_1 = \beta_1 \\ c_1 = \beta_2 \\ d_1 = \beta_3$
\section*{b)}
$f_2(x) = a_2 + b_2x + c_2x^2 + d_2x^3 \ \ x>\xi$ \newline
if $x > \xi$ then $(x - \xi)^3_+ = ( x - \xi)^3$ by definition. \newline
Thus $f(x) = \beta_0 + \beta_1x + \beta_2x^2+\beta_3 x^3 + \beta_4(x - \xi)^3 = \\
= \beta_0 + \beta_1x + \beta_2x^2 + \beta_3x^3 + \beta_4(x^3 - \xi^3 -3x^2\xi + 3x\xi^2) = \\
= \beta_0 - \beta_4\xi^3 + x(\beta_1 + 3\beta_4\xi^2) + x^2(\beta_2 - 3\beta_4\xi) + x^3(\beta_3 + \beta_4) \\$
And we set: \newline
$a_2 = \beta_0 - \beta_4\xi^3 \\ b_2 = \beta_1 + 3\beta_4\xi^2 \\ c_2 = \beta_2 - 3\beta_4\xi \\ d_2 = \beta_3 + \beta_4$
\section*{c)}
$\lim\limits_{x\xrightarrow{}\xi}f_2(x) = \lim\limits_{x\xrightarrow{}\xi}\beta_0 - \beta_4\xi^3 + x(\beta_1 + 3\beta_4\xi^2) + x^2(\beta_2 - 3\beta_4\xi) + x^3(\beta_3 + \beta_4) = \beta_0 - \beta_4\xi^3 + \xi(\beta_1 + 3\beta_4\xi^2) + \xi^2(\beta_2 - 3\beta_4\xi)  + \xi^3(\beta_3 + \beta_4) = \beta_0 + \beta_1\xi + \beta_2\xi^2 + \beta_3\xi^3 = \\ = \lim\limits_{x\xrightarrow{}\xi}f_1(x)$. \newline
Hence $f$ is continuous in $\xi$.
\section*{d)}
$f_1^{'}(x) = \beta_1 + 2\beta_2x + 3\beta_3x^2$ and \\ $f_2^{'}(x) = \beta_1 + 3\beta_4\xi^2 + 2x(\beta_2 - 3\beta_4\xi) + 3x^2(\beta_3 + \beta_4)$\vspace{0.3 cm}\newline
$\lim\limits_{x \xrightarrow{}\xi}f_2^{'}(x) = \beta_1 + 3\beta_4\xi^2 + 2\xi(\beta_2 - 3\beta_4\xi) + 3\xi^2(\beta_3 + \beta_4) = \beta_1 + 2\beta_2\xi + 3\beta_3\xi^2 = \\
 = \lim\limits_{x\xrightarrow{}\xi}f_1^{'}(x)$
 \section*{e)}
$f_1^{''}(x) = 2\beta_2 + 6\beta_3x$ and \\ $f_2^{''}(x) = 2(\beta_2 - 3\beta_4\xi) + 6x(\beta_3 + \beta_4)$\vspace{0.3 cm}\newline
$\lim\limits_{x \xrightarrow{}\xi}f_2^{''}(x) =  2(\beta_2 - 3\beta_4\xi) + 6\xi(\beta_3 + \beta_4) = 2\beta_2 + 6\beta_3\xi = \lim\limits_{x \xrightarrow{}\xi}f_1^{''}(x)$
\section*{2}

% not sure of a and b
\section*{a)} $\hat{g_1}$ will have smaller training RSS because is less regular than $\hat{g_1}$ and will fit the training data better (i.e. small bias).
\section*{b)} $\hat{g_2}$ will have smaller test RSS because is more regular and less sensitive to over-fitting.
\section*{c)} For $\lambda = 0$ $\hat{g}_1 = \hat{g}_2$ and RSS on train is equal to zero because the function $g$ will be an interpolation function of the given points.
\end{document} 
