\documentclass[12pt]{article}
\usepackage{graphicx} % Required for inserting images
\usepackage{amsmath}
\usepackage{amssymb}
\usepackage[italian]{babel}
\usepackage{hyperref}%
\usepackage{mathrsfs}



\begin{document}


\section*{}
Marco Reina 7066486 \newline
Samuele Serri 7069839 \newline
\section*{a)}
Given: 
\begin{equation*}
    l(\beta) = \sum_{i = 1}^ny_i\log\Big(\frac{e^{f(x_i;\beta)}}{1 + e^{f(x_i;\beta)}}\Big) + (1 - y_i)log\Big(1 - \frac{e^{f(x_i;\beta)}}{1 + e^{f(x_i;\beta)}}\Big)
\end{equation*}
We compute $\nabla_\beta l(\beta)$ as:
\begin{equation*}
    \nabla_\beta l(\beta) = \nabla_\beta\sum_{i = 1}^ny_i\Big[f({x_i;\beta) - log(1 + e^{f(x_i;\beta)})}\Big] + (1 - y_i)(-log(1 + e^{f(x_i;\beta)})) = 
\end{equation*}
\begin{equation*}
    = \nabla_\beta\sum_{i = 1}^ny_i f(x_i;\beta) - y_i log(1 + e^{f(x_i;\beta)}) + y_i log(1 + e^{f(x_i;\beta)}) - log(1 + e^{f(x_i;\beta)}) = 
\end{equation*}
\begin{equation*}
    = \nabla_\beta\sum_{i = 1}^n y_i f(x_i; \beta) - log( 1 + e^{f(x_i;\beta)}) = 
\end{equation*}
\begin{equation*}
    = \sum_{i = 1}^n y_i\nabla_\beta f(x_i; \beta) - \frac{e^{f(x_i;\beta)}\nabla_\beta f(x_i; \beta)}{1 + e^{f(x_i;\beta)}}
\end{equation*}
if $f(x_i; \beta) = \beta_0 + x_{i1}\beta_1 + x_{i2}\beta_2$ then:
\begin{equation*}
    \nabla_\beta f(x_i; \beta) = \begin{pmatrix}
        1 \\ x_{i1} \\ x_{i2}
    \end{pmatrix}
\end{equation*}
and 
\begin{equation*}
    \nabla_\beta l(\beta) =  \begin{pmatrix}
        \partial_{\beta_0}l(\beta) \\
        \partial_{\beta_1}l(\beta) \\
        \partial_{\beta_2}l(\beta) \\
    \end{pmatrix}= \begin{pmatrix}
        \sum_{i = 1}^n y_i - \frac{e^{f(x_i;\beta)}}{1 + e^{f(x_i;\beta)}} \\
        \sum_{i = 1}^n y_i x_{i1} - \frac{e^{f(x_i;\beta)}x_{i1}}{1 + e^{f(x_i;\beta)}} \\
        \sum_{i = 1}^n y_i x_{i2} - \frac{e^{f(x_i;\beta)}x_{i2}}{1 + e^{f(x_i;\beta)}} 
    \end{pmatrix}
\end{equation*}
\section*{b)}
\section*{c)}
\end{document}
